coq/JsPreliminaryAux.v
@@ -341,17 +341,18 @@ Proof. introv. typeclass. Qed.
 
 (** Decidable instance for [is_callable] *)
 
-Definition run_callable S v : option call :=
+Definition run_callable S v : option (option call) :=
   match v with
-  | value_prim w => None
-  | value_object l => morph_option None object_call_ (pick_option (object_binds S l))
+  | value_prim w => Some None
+  | value_object l =>
+    morph_option None (fun O => Some (object_call_ O)) (pick_option (object_binds S l))
   end.
 
 Global Instance is_callable_dec : forall S v,
   Decidable (is_callable S v).
 Proof.
   introv. applys decidable_make
-    (morph_option false (fun _ => true) (run_callable S v)).
+    (morph_option false (morph_option false (fun _ => true)) (run_callable S v)).
   destruct v; simpl.
    fold_bool. rewrite is_False with (P := is_callable _ _). rewrite* isTrue_false.
     intro A. do 2 inverts A as A.
